coq/ExtractProofState.v
@@ -8,13 +8,14 @@ From Coq Require Import
   Extraction ExtrOcamlBasic ExtrOcamlNatInt ExtrOcamlNativeString.
 From ZFCert Require Import
   ProofState TacticCompleteness ZFC NamedProofState NamedCommands
-  CertifiedSession.
+  CertifiedSession GlobalEnvironment.
 
 Extraction Language OCaml.
 Set Extraction Output Directory "extracted".
 Extraction "proof_state.ml"
-  start state_goals
+  start_with_assumptions start state_goals
   step run rule_step rule_run
+  named_start_with_environment
   named_start_with_constants named_start named_goals named_solved
   named_step named_run named_rule_step named_rule_run
   named_default_all_intro_rule_step
@@ -24,13 +25,17 @@ Extraction "proof_state.ml"
   named_separation_tactic_step
   named_replacement_tactic_step
   named_execute_rule
+  certified_start_with_environment
   certified_start_with_constants certified_start certified_goals certified_solved
   one_step certified_step certified_run
   certified_certificate
+  replay_certificate_with_environment
   replay_certificate_with_constants replay_certificate certified_finalize
   certified_execute_rule
   certified_separation_tactic
   certified_replacement_tactic
+  empty_global_environment global_fact_names global_start global_replay
+  global_declare_choice
   empty_set_axiom extensionality_axiom pairing_axiom union_axiom
   power_set_axiom foundation_axiom infinity_axiom choice_axiom
   separation_instance replacement_instance.
